{
 "cells": [
  {
   "cell_type": "code",
   "execution_count": null,
   "metadata": {},
   "outputs": [],
   "source": []
  },
  {
   "cell_type": "markdown",
   "metadata": {},
   "source": [
    "# mandatory assignment 1 questions\n",
    "## Exact solution\n",
    "We define\n",
    "$$\n",
    "u(t,x,y) = e^{\\imath(k_xx + k_y y - \\omega t)}.\n",
    "$$\n",
    "we compute $\\frac{\\partial^2 u}{\\partial x^2}$:\n",
    "$$\n",
    "\\frac{\\partial^2 u}{\\partial x^2} = -k_x^2 e^{\\imath(k_xx + k_y y - \\omega t)} = -k_x^2 u(t,x,y),\n",
    "$$\n",
    "and equivalently for  $\\frac{\\partial^2 u}{\\partial y^2}$:\n",
    "$$\n",
    "\\frac{\\partial^2 u}{\\partial y^2} = -k_y^2 u(x,x,y),\n",
    "$$\n",
    "as such:\n",
    "$$\n",
    "\\nabla^2 u = \\frac{\\partial^2 u}{\\partial x^2} + \\frac{\\partial^2 u}{\\partial y^2}\n",
    "= -(k_x^2 + k_y^2)u.\n",
    "$$\n",
    "We compute $\\frac{\\partial^2 u }{\\partial t^2}$:\n",
    "$$\n",
    "\\frac{\\partial^2 u }{\\partial t^2} = -\\omega^2 u.\n",
    "$$\n",
    "we state the wave equation:\n",
    "$$\n",
    "\\frac{\\partial^2 u }{\\partial t^2} = c^2 \\nabla^2 u\\\\ \n",
    "\\Rightarrow  -\\omega^2 u = c^2 (-(k_x^2 + k_y^2)u)\n",
    "$$\n",
    "since $\\omega$, $c$, $k_x$ and $k_y$ are constants, this is not contradictory, hence the equation is satisfied.\n",
    "## Dispersion coefficient\n",
    "we now assume $k_x = k_y = k$ and $m_x = m_y$. we discretize\n",
    "$$\n",
    "u(t,x,y) = e^{\\imath(k_xx + k_y y - \\omega t)},\n",
    "$$\n",
    "as such:\n",
    "$$\n",
    "u_{ij}^n = e^{\\imath (kh(i+j) - \\bar{\\omega}n\\Delta t)}\n",
    "$$\n",
    "\n",
    "we plugin into \n",
    "\\begin{equation}\n",
    "\\frac{u^{n+1}_{i,j} - 2u^n_{i,j} + u^{n-1}_{i, j}}{\\Delta t^2} =\n",
    " c^2 \\left(\\frac{u^n_{i+1,j} - 2u^n_{i,j} + u^n_{i-1, j}}{h^2} + \\frac{u^n_{i,j+1} - 2u^n_{i,j} + u^n_{i, j-1}}{h^2}\\right)\n",
    "\\end{equation}\n",
    "as such:\n",
    "\\begin{align}\n",
    "&\\frac{e^{\\imath (kh(i+j) - \\bar{\\omega}(n+1)\\Delta t)} - 2e^{\\imath (kh(i+j) - \\bar{\\omega}n\\Delta t)} + e^{\\imath (kh(i+j) - \\bar{\\omega}(n-1)\\Delta t)}}{\\Delta t^2} =\\\\\n",
    " &c^2 \\left(\\frac{e^{\\imath (kh(i+j+1) - \\bar{\\omega}n\\Delta t)} - 2e^{\\imath (kh(i+j) - \\bar{\\omega}n\\Delta t)} + e^{\\imath (kh(i+j - 1) - \\bar{\\omega}n\\Delta t)}}{h^2} + \\frac{e^{\\imath (kh(i+j+1) - \\bar{\\omega}n\\Delta t)} - 2e^{\\imath (kh(i+j) - \\bar{\\omega}n\\Delta t)} + e^{\\imath (kh(i+j-1) - \\bar{\\omega}n\\Delta t)}}{h^2}\\right)\n",
    "\\end{align}\n",
    "bto\n",
    "\\begin{align}\n",
    "\\Rightarrow\n",
    "&\\frac{e^{\\imath (kh(i+j) - \\bar{\\omega}(n+1)\\Delta t)} - 2e^{\\imath (kh(i+j) - \\bar{\\omega}n\\Delta t)} + e^{\\imath (kh(i+j) - \\bar{\\omega}(n-1)\\Delta t)}}{\\Delta t^2} =\\\\\n",
    " &2c^2 \\left(\\frac{e^{\\imath (kh(i+j+1) - \\bar{\\omega}n\\Delta t)} - 2e^{\\imath (kh(i+j) - \\bar{\\omega}n\\Delta t)} + e^{\\imath (kh(i+j - 1) - \\bar{\\omega}n\\Delta t)}}{h^2}\\right)\n",
    "\\end{align}\n",
    "lol\n",
    "\\begin{align}\n",
    "\\Rightarrow\n",
    "&e^{\\imath (kh(i+j) - \\bar{\\omega}n\\Delta t)}\\frac{e^{\\imath (-\\bar{\\omega}\\Delta t)} - 2 + e^{\\imath (- \\bar{\\omega}(-1)\\Delta t)}}{\\Delta t^2} =\\\\\n",
    " &e^{\\imath (kh(i+j) - \\bar{\\omega}n\\Delta t)}2c^2 \\left(\\frac{e^{\\imath (kh(1))} - 2 + e^{\\imath (kh(- 1))}}{h^2}\\right)\n",
    "\\end{align}\n",
    "eh\n",
    "\\begin{align}\n",
    "\\Rightarrow\n",
    "&\\frac{2\\cos{\\bar{\\omega}\\Delta t} - 2}{\\Delta t^2} =\\\\\n",
    " &2c^2 \\left(\\frac{2\\cos{kh} - 2}{h^2}\\right)\n",
    "\\end{align}\n",
    "continuing:\n",
    "\\begin{align}\n",
    "\\Rightarrow\n",
    "&\\frac{\\cos{\\bar{\\omega}\\Delta t} - }{\\Delta t^2} =\\\\\n",
    " &2c^2 \\left(\\frac{\\cos{kh} - 1}{h^2}\\right)\n",
    "\\end{align}\n",
    "ehm\n",
    "\\begin{align}\n",
    "\\Rightarrow\n",
    "&\\cos{\\bar{\\omega}\\Delta t} - 1 =\n",
    " &\\frac{2c^2 \\Delta t^2}{h^2} \\left(\\cos{kh} - 1\\right)\n",
    "\\end{align}\n",
    "CFL is defined as follows:\n",
    "$$\n",
    "C = \\frac{c \\Delta t}{h}\n",
    "$$\n",
    "if we set $C = \\frac{1}{\\sqrt{2}}$, as such: $C^2 = \\frac{1}{2}$ which would require $\\frac{c^2 \\Delta t^2}{h^2} = \\frac{1}{2}$ as such:\n",
    "\\begin{align}\n",
    "\\Rightarrow\n",
    "&\\cos{\\bar{\\omega}\\Delta t} - 1 =\n",
    "\\cos{kh} - 1\n",
    "\\end{align}\n",
    "and $\\bar{\\omega}\\Delta t = kh$. Truthfully im not sure how to extend this such that $\\bar{\\omega} = \\omega$"
   ]
  }
 ],
 "metadata": {
  "language_info": {
   "name": "python"
  }
 },
 "nbformat": 4,
 "nbformat_minor": 2
}
